experiment/Experiment.Steel.SteelHack.fst
@@ -1,0 +1,84 @@
+module Experiment.Steel.SteelHack
+
+open FStar.Tactics
+
+let intro_conj_with_impl (#a #b : Type0)
+  : Lemma (requires a /\ (a ==> b)) (ensures a /\ b)
+  = ()
+
+let intro_subcomp_pre'
+  (#a:Type)
+  (#pre_f:pre_t) (#post_f:post_t a) (req_f:req_t pre_f) (ens_f:ens_t pre_f a post_f)
+  (#pre_g:pre_t) (#post_g:post_t a) (req_g:req_t pre_g) (ens_g:ens_t pre_g a post_g)
+  (#frame:vprop)
+  (#pr:prop)
+  p1 p2 s_pr s_pre s_post
+  : subcomp_pre' req_f ens_f req_g ens_g p1 p2
+  = 
+    let cbst_pre          = can_be_split_trans pre_g      (pre_f    `star` frame) in
+    let cbst_post (x : a) = can_be_split_trans (post_g x) (post_f x `star` frame) in
+    _ by (
+    set_guard_policy Force;
+    norm [delta_only [`%subcomp_pre']];
+    split ();
+
+    let h0   = forall_intro () in
+    let rq_g = implies_intro () in
+    apply_lemma (`intro_conj_with_impl); split ();
+    apply_lemma (`(`@s_pr)); exact h0; hyp rq_g;
+    let h_pr = implies_intro () in
+    apply_lemma (`(`@s_pre)); explode ();
+    hyp rq_g;
+    hyp h_pr;
+    apply_lemma (`(`@cbst_pre)); smt ();
+
+    let h0 = forall_intro () in
+    let x  = forall_intro () in
+    let h1 = forall_intro () in
+    let h_pr = implies_intro () in
+    let _hs0  = implies_intro () in
+    let _hs1,eq_fr  = destruct_and _hs0 in
+    clear _hs0;
+    let rq_g, en_f = destruct_and _hs1 in
+    clear _hs1;
+    apply_lemma (`(`@s_post));
+    explode ();
+    hyp rq_g;
+    hyp h_pr;
+    apply_lemma (`(`@cbst_pre)); smt ();
+    apply_lemma (`(`@cbst_post)); smt ();
+    apply_lemma (`can_be_split_interp); apply_lemma (`(`@cbst_pre));  smt ();
+    apply_lemma (`can_be_split_interp); apply_lemma (`(`@cbst_post)); smt ();
+    hyp en_f;
+    hyp eq_fr
+  )
+
+
+/// Modified version of [init_resolve_tac]
+[@@ resolve_implicits; framing_implicit]
+let resolve_framing () : Tac unit =
+  let slgs, loggs = filter_goals (goals()) in
+  set_goals slgs;
+  solve_maybe_emps (goals ());
+  solve_indirection_eqs (goals());
+
+  //Solve the two goals using the hypothesis p1, p2
+  let _ = repeatn 2 begin fun () ->
+    first (map (fun (b : binder) -> fun () -> exact b <: Tac unit) (cur_binders ()))
+  end in
+  
+  set_goals loggs;
+  resolve_tac_logical ()
+
+[@@ handle_smt_goals ]
+let tac () =
+  first (map (fun (b : binder) -> fun () -> (
+    if term_to_string b <> "sc" then fail "";
+    norm_binder_type [delta_only [`%subcomp_pre']] b;
+    norm_binder_type normal_steps b;
+    exact b
+  ) <: Tac unit) (cur_binders ()))
+
+inline_for_extraction
+let steel_subcomp a pre_f post_f req_f ens_f pre_g post_g req_g ens_g frame pr p1 p2 sc $f ()
+  = f ()
