experiment/Experiment.Steel.SteelHack.fsti
@@ -1,0 +1,84 @@
+module Experiment.Steel.SteelHack
+
+module Mem = Steel.Memory
+
+open Steel.Effect
+
+type unit_steel (a : Type) (pre : pre_t) (post : post_t a) (req : req_t pre) (ens : ens_t pre a post)
+  = unit -> Steel a pre post req ens
+
+/// [subcomp_pre] without [rewrite_with_tactic] and [frame_equality] reduced
+let subcomp_pre' (#a:Type)
+  (#pre_f:pre_t) (#post_f:post_t a) (req_f:req_t pre_f) (ens_f:ens_t pre_f a post_f)
+  (#pre_g:pre_t) (#post_g:post_t a) (req_g:req_t pre_g) (ens_g:ens_t pre_g a post_g)
+  (#frame:vprop)
+  (#pr:prop)
+  (_:squash (can_be_split_dep pr pre_g (pre_f `star` frame)))
+  (_:squash (equiv_forall post_g (fun x -> post_f x `star` frame)))
+  : pure_pre
+= squash (
+  (forall (h0:hmem pre_g). req_g (mk_rmem pre_g h0) ==> pr /\
+    (can_be_split_trans pre_g (pre_f `star` frame) pre_f;
+    req_f (focus_rmem (mk_rmem pre_g h0) pre_f))) /\
+  (forall (h0:hmem pre_g) (x:a) (h1:hmem (post_g x)). (
+     pr ==> (
+     can_be_split_trans (post_g x) (post_f x `star` frame) (post_f x);
+     can_be_split_trans (pre_g) (pre_f `star` frame) frame;
+     can_be_split_trans (post_g x) (post_f x `star` frame) frame;
+     can_be_split_trans pre_g (pre_f `star` frame) pre_f;
+
+     (req_g (mk_rmem pre_g h0) /\
+      ens_f (focus_rmem (mk_rmem pre_g h0) pre_f) x (focus_rmem (mk_rmem (post_g x) h1) (post_f x)) /\
+      (*
+      frame_equalities frame
+        (focus_rmem (mk_rmem pre_g h0) frame)
+        (focus_rmem (mk_rmem (post_g x) h1) frame)*)
+      sel_of frame
+        (let _ = can_be_split_interp pre_g (pre_f `star` frame) h0 in h0) ==
+      sel_of frame
+        (let _ = can_be_split_interp (post_g x) (post_f x `star` frame) h1 in h1)
+     )
+        ==> ens_g (mk_rmem pre_g h0) x (mk_rmem (post_g x) h1))
+  ))
+)
+
+val intro_subcomp_pre'
+  (#a:Type)
+  (#pre_f:pre_t) (#post_f:post_t a) (req_f:req_t pre_f) (ens_f:ens_t pre_f a post_f)
+  (#pre_g:pre_t) (#post_g:post_t a) (req_g:req_t pre_g) (ens_g:ens_t pre_g a post_g)
+  (#frame:vprop)
+  (#pr:prop)
+  (p1:squash (can_be_split_dep pr pre_g (pre_f `star` frame)))
+  (p2:squash (equiv_forall post_g (fun x -> post_f x `star` frame)))
+  (s_pr   : (h0:hmem pre_g) -> Lemma
+     (requires req_g (mk_rmem pre_g h0))
+     (ensures  pr))
+  (s_pre  : (h0:hmem pre_g) -> Lemma
+     (requires req_g (mk_rmem pre_g h0) /\ pr /\
+               can_be_split pre_g pre_f)
+     (ensures  req_f (focus_rmem (mk_rmem pre_g h0) pre_f)))
+  (s_post : (h0:hmem pre_g) -> (x:a) -> (h1:hmem (post_g x)) -> Lemma
+     (requires req_g (mk_rmem pre_g h0) /\ pr /\
+               can_be_split pre_g pre_f /\
+               can_be_split (post_g x) (post_f x) /\
+               Mem.interp (hp_of frame) h0 /\
+               Mem.interp (hp_of frame) h1 /\
+               ens_f (focus_rmem (mk_rmem pre_g h0) pre_f) x (focus_rmem (mk_rmem (post_g x) h1) (post_f x)) /\
+               sel_of frame h0 == sel_of frame h1)
+     (ensures  ens_g (mk_rmem pre_g h0) x (mk_rmem (post_g x) h1)))
+  : subcomp_pre' req_f ens_f req_g ens_g p1 p2
+
+
+inline_for_extraction
+val steel_subcomp (a:Type)
+  (pre_f:pre_t)       (post_f:post_t a)
+  (req_f:req_t pre_f) (ens_f:ens_t pre_f a post_f)
+  (pre_g:pre_t)       (post_g:post_t a)
+  (req_g:req_t pre_g) (ens_g:ens_t pre_g a post_g)
+  (frame:vprop)
+  (pr : prop)
+  (p1 : squash (can_be_split_dep pr pre_g (pre_f `star` frame)))
+  (p2 : squash (equiv_forall post_g (fun x -> post_f x `star` frame)))
+  (sc : squash (subcomp_pre' req_f ens_f req_g ens_g p1 p2))
+  ($f : unit_steel a pre_f post_f req_f ens_f)
+  : unit_steel a pre_g post_g req_g ens_g
